feat: enum

TestModels/SimpleTypes/SimpleEnum/src/SimpleEnumImpl.dfy
@@ -10,9 +10,58 @@ module SimpleEnumImpl refines AbstractSimpleTypesEnumOperations  {
   predicate GetEnumEnsuresPublicly(input: GetEnumInput, output: Result<GetEnumOutput, Error>) {
     true
   }
+  predicate GetEnumFirstKnownValueTestEnsuresPublicly(input: GetEnumInput, output: Result<GetEnumOutput, Error>) {
+    true
+  }
+  predicate GetEnumSecondKnownValueTestEnsuresPublicly(input: GetEnumInput, output: Result<GetEnumOutput, Error>) {
+    true
+  }
+  predicate GetEnumThirdKnownValueTestEnsuresPublicly(input: GetEnumInput, output: Result<GetEnumOutput, Error>) {
+    true
+  }
   method GetEnum ( config: InternalConfig,  input: GetEnumInput )
   returns (output: Result<GetEnumOutput, Error>) {
     var res := GetEnumOutput(value := input.value);
+    return Success(res);
+  }
+
+  // Known value tests. See "Known value test" in TestModels' README.
+  method GetEnumFirstKnownValueTest ( config: InternalConfig,  input: GetEnumInput )
+  returns (output: Result<GetEnumOutput, Error>) {
+    expect input.value.Some?;
+    expect input.value.value == FIRST;
+
+    var res := GetEnumOutput(value := input.value);
+
+    expect res.value.Some?;
+    expect res.value.value == FIRST; 
+
+    return Success(res);
+  }
+
+  method GetEnumSecondKnownValueTest ( config: InternalConfig,  input: GetEnumInput )
+  returns (output: Result<GetEnumOutput, Error>) {
+    expect input.value.Some?;
+    expect input.value.value == SECOND;
+
+    var res := GetEnumOutput(value := input.value);
+
+    expect res.value.Some?;
+    expect res.value.value == SECOND; 
+    
+    return Success(res);
+  }
+
+  method GetEnumThirdKnownValueTest ( config: InternalConfig,  input: GetEnumInput )
+  returns (output: Result<GetEnumOutput, Error>) {
+    expect input.value.Some?;
+    expect input.value.value == THIRD;
+
+    var res := GetEnumOutput(value := input.value);
+
+    expect res.value.Some?;
+    expect res.value.value == THIRD; 
+    
     return Success(res);
   }
 }
