TestModels/SimpleTypes/SimpleEnum/test/SimpleEnumImplTest.dfy
@@ -8,6 +8,9 @@ module  SimpleEnumImplTest {
     method{:test} GetEnum(){
         var client :- expect SimpleEnum.SimpleEnum();
         TestGetEnum(client);
+        TestGetEnumFirstKnownValueTest(client);
+        TestGetEnumSecondKnownValueTest(client);
+        TestGetEnumThirdKnownValueTest(client);
     }
 
     // TODO: Add more tests once we can run SimpleEnum tests
@@ -17,7 +20,60 @@ module  SimpleEnumImplTest {
       modifies client.Modifies
       ensures client.ValidState()
     {
-        var ret := client.GetEnum(SimpleEnum.Types.GetEnumInput(value:= Some(THIRD)));
+        var convertedEnumInput := SimpleEnum.Types.GetEnumInput(value:= Some(THIRD));
+        
+        expect convertedEnumInput.value.value == THIRD;
+
+        var ret := client.GetEnum(convertedEnumInput);
+        
+        expect ret.Success?;
+        expect ret.value.value.UnwrapOr(FIRST) == THIRD;
+        print ret;
+    }
+
+    method TestGetEnumFirstKnownValueTest(client: ISimpleTypesEnumClient)
+      requires client.ValidState()
+      modifies client.Modifies
+      ensures client.ValidState()
+    {
+        var convertedEnumInput := SimpleEnum.Types.GetEnumInput(value:= Some(FIRST));
+        
+        expect convertedEnumInput.value.value == FIRST;
+
+        var ret := client.GetEnumFirstKnownValueTest(convertedEnumInput);
+        
+        expect ret.Success?;
+        expect ret.value.value.UnwrapOr(THIRD) == FIRST;
+        print ret;
+    }
+
+    method TestGetEnumSecondKnownValueTest(client: ISimpleTypesEnumClient)
+      requires client.ValidState()
+      modifies client.Modifies
+      ensures client.ValidState()
+    {
+        var convertedEnumInput := SimpleEnum.Types.GetEnumInput(value:= Some(SECOND));
+        
+        expect convertedEnumInput.value.value == SECOND;
+
+        var ret := client.GetEnumSecondKnownValueTest(convertedEnumInput);
+        
+        expect ret.Success?;
+        expect ret.value.value.UnwrapOr(THIRD) == SECOND;
+        print ret;
+    }
+
+    method TestGetEnumThirdKnownValueTest(client: ISimpleTypesEnumClient)
+      requires client.ValidState()
+      modifies client.Modifies
+      ensures client.ValidState()
+    {
+        var convertedEnumInput := SimpleEnum.Types.GetEnumInput(value:= Some(THIRD));
+        
+        expect convertedEnumInput.value.value == THIRD;
+
+        var ret := client.GetEnumThirdKnownValueTest(convertedEnumInput);
+        
         expect ret.Success?;
         expect ret.value.value.UnwrapOr(FIRST) == THIRD;
         print ret;
